more rec lang

theories/module.v
@@ -312,6 +312,140 @@ Proof.
   eexists. by apply: link_trace_related_step.
 Qed.
 
+(*** has_non_ub_trace *)
+Inductive has_non_ub_trace {EV} (m : module EV) : m.(m_state) → list EV → m.(m_state) → Prop :=
+| NUBTraceEnd σ:
+    has_non_ub_trace m σ [] σ
+| NUBTraceStep σ1 σ2 σ3 κ κs:
+    m.(m_step) σ1 κ σ2 →
+    has_non_ub_trace m σ2 κs σ3 →
+    has_non_ub_trace m σ1 (option_list κ ++ κs) σ3
+.
+
+Lemma NUBTraceStepNone {EV} κs (m : module EV) σ2 σ1 σ3 :
+  m.(m_step) σ1 None σ2 →
+  has_non_ub_trace m σ2 κs σ3 →
+  has_non_ub_trace m σ1 κs σ3.
+Proof. move => ??. by apply: (NUBTraceStep _ _ _ _ None). Qed.
+
+Lemma NUBTraceStepSome {EV} κs (m : module EV) σ2 σ1 σ3 κ :
+  m.(m_step) σ1 (Some κ) σ2 →
+  has_non_ub_trace m σ2 κs σ3 →
+  has_non_ub_trace m σ1 (κ :: κs) σ3.
+Proof. move => ??. by apply: (NUBTraceStep _ _ _ _ (Some _)). Qed.
+
+Lemma has_non_ub_trace_trans {EV} κs1 κs2 (m : module EV) σ1 σ2 σ3 :
+  has_non_ub_trace m σ1 κs1 σ2 →
+  has_non_ub_trace m σ2 κs2 σ3 →
+  has_non_ub_trace m σ1 (κs1 ++ κs2) σ3.
+Proof.
+  elim => //.
+  move => ?????????. rewrite -app_assoc. econstructor; eauto.
+Qed.
+
+Lemma has_non_ub_trace_add_empty {EV} κs1 (m : module EV) σ1 σ2 :
+  has_non_ub_trace m σ1 (κs1 ++ []) σ2 →
+  has_non_ub_trace m σ1 κs1 σ2.
+Proof. by rewrite -{2}[κs1](right_id_L [] (++)). Qed.
+
+(*** has_no_behavior *)
+Definition has_no_behavior {EV} (m : module EV) (σ : m.(m_state)) :=
+  ∀ σ' κs, has_trace m σ κs σ' → κs = [].
+
+Lemma no_behavior_step {EV} (m : module EV) σ:
+  (∀ e σ', m.(m_step) σ e σ' → e = None ∧ has_no_behavior m σ') → ¬(m_is_ub m σ) → has_no_behavior m σ.
+Proof. move => Hstep ??? Htrace. inversion Htrace; simplify_eq/= => //. efeed pose proof Hstep => //. naive_solver. Qed.
+
+(*** state_set *)
+Definition state_set_refines {EV} (mimpl mspec : module EV) (σi : mimpl.(m_state)) (σs : propset mspec.(m_state)) : Prop :=
+  ∀ κs σi2, has_trace mimpl σi κs σi2 → ∃ σs1 σs2, σs1 ∈ σs ∧ has_trace mspec σs1 κs σs2.
+
+Lemma inv_set_implies_refines {EV} (m1 m2 : module EV) (inv : m1.(m_state) → propset m2.(m_state) → Prop):
+  inv m1.(m_initial) {[ m2.(m_initial) ]} →
+  (∀ σi σs, inv σi σs → ∃ σ, σ ∈ σs) →
+  (∀ σi σs, inv σi σs → m1.(m_is_ub) σi → ∃ σs1 σs2, σs1 ∈ σs ∧ has_trace m2 σs1 [Ub] σs2) →
+  (∀ σi1 σs1 σi2 e, inv σi1 σs1 → m1.(m_step) σi1 e σi2 →
+      ∃ σs2, inv σi2 σs2 ∧ σs2 ⊆ {[ σ2 | ∃ σ1, σ1 ∈ σs1 ∧ has_trace m2 σ1 (option_list (Vis <$> e)) σ2 ]}) →
+  refines m1 m2.
+Proof.
+  move => Hinvinit Hinvnonempty Hinvsafe Hinvstep.
+  constructor => // κs σi2.
+  move: m1.(m_initial) Hinvinit => σi1 Hinv Hsteps.
+  have : (∃ σs1 σs2, σs1 ∈ ({[m_initial m2]} : propset _) ∧ has_trace m2 σs1 κs σs2); last set_solver.
+  move: {[ m2.(m_initial) ]} Hinv => σs1 Hinv.
+  elim: Hsteps σs1 Hinv => {σi1 σi2 κs}.
+  - move => ? ? /Hinvnonempty [??].  eexists _, _. split => //. by apply: TraceEnd.
+  - move => σi1 σi2 σi3 κ κs Hstep Hsteps IH σs1 Hinv.
+    have [σs2 [Hinv2 Hsub]]:= Hinvstep _ _ _ _ Hinv Hstep.
+    have [σs3 [σs4 [Hin ?]]]:= IH _ Hinv2.
+    have [σ1 [??]]:= Hsub _ Hin.
+    eexists _, _. split => //. by apply: has_trace_trans.
+  - move => ??? /Hinvsafe Hs σs Hinv.
+    have [? [? [? /has_trace_ub_inv[σs2[??]]]]]:= Hs _ Hinv.
+    eexists _, _. split => //. apply: (has_trace_trans []); [ done |]. by apply: TraceUbRefl.
+Qed.
+
+Lemma state_set_refines_initial {EV} (m1 m2 : module EV):
+  refines m1 m2 →
+  state_set_refines m1 m2 (m_initial m1) {[m_initial m2]}.
+Proof. move => [Hr] ?? /Hr[??]. naive_solver. Qed.
+
+Lemma state_set_refines_step {EV} (m1 m2 : module EV) σi1 σs1 σi2 e:
+  state_set_refines m1 m2 σi1 σs1 →
+  m1.(m_step) σi1 e σi2 →
+  state_set_refines m1 m2 σi2 {[ σ2 | ∃ σ1, σ1 ∈ σs1 ∧ has_trace m2 σ1 (option_list (Vis <$> e)) σ2 ]}.
+Proof.
+  move => Hinv Hstep κs σi3 Hκs.
+  have [|? [? [? /has_trace_app_inv[?[??]]]]]:= Hinv (option_list (Vis <$> e) ++ κs) σi3.
+  { by apply: TraceStep. }
+  set_solver.
+Qed.
+
+Lemma state_set_refines_step_None {EV} (m1 m2 : module EV) σi1 σs1 σi2:
+  state_set_refines m1 m2 σi1 σs1 →
+  m1.(m_step) σi1 None σi2 →
+  state_set_refines m1 m2 σi2 σs1.
+Proof.
+  move => Hinv Hstep κs σi3 Hκs.
+  have [|? [? [? ?]]]:= Hinv κs σi3.
+  { by apply: TraceStepNone. }
+  set_solver.
+Qed.
+
+Lemma state_set_refines_non_empty {EV} (m1 m2 : module EV) σi σs:
+  state_set_refines m1 m2 σi σs → ∃ σ, σ ∈ σs.
+Proof.
+  move => Hs.
+  have [|?[?[??]]]:= Hs [] σi. by apply: TraceEnd.
+  naive_solver.
+Qed.
+
+Lemma state_set_refines_ub {EV} (m1 m2 : module EV) σi σs:
+  state_set_refines m1 m2 σi σs →
+  m1.(m_is_ub) σi →
+  ∃ σ σ', σ ∈ σs ∧ has_trace m2 σ [Ub] σ'.
+Proof. move => Hs Hub. apply: Hs. by apply: TraceUbRefl. Qed.
+
+Lemma refines_implies_inv_set {EV} (m1 m2 : module EV):
+  refines m1 m2 →
+  ∃ (inv : m1.(m_state) → propset m2.(m_state) → Prop),
+  inv m1.(m_initial) {[ m2.(m_initial) ]} ∧
+  (∀ σi σs, inv σi σs → ∃ σ, σ ∈ σs) ∧
+  (∀ σi σs, inv σi σs → m1.(m_is_ub) σi → ∃ σs1 σs2, σs1 ∈ σs ∧ has_trace m2 σs1 [Ub] σs2) ∧
+  (∀ σi1 σs1 σi2 e, inv σi1 σs1 → m1.(m_step) σi1 e σi2 →
+      ∃ σs2, inv σi2 σs2 ∧ σs2 ⊆ {[ σ2 | ∃ σ1, σ1 ∈ σs1 ∧ has_trace m2 σ1 (option_list (Vis <$> e)) σ2 ]}).
+Proof.
+  move => Href.
+  eexists (state_set_refines m1 m2).
+  split_and!.
+  - by apply: state_set_refines_initial.
+  - by apply: state_set_refines_non_empty.
+  - move => σi σs Hinv Hub. by apply: state_set_refines_ub.
+  - move => σi1 σs1 σi2 e Hinv Hstep.
+    eexists _. split_and!; last reflexivity.
+    by apply: state_set_refines_step.
+Qed.
+
 (*** wp': equivalent definition of refines *)
 Inductive wp' {EV} (m1 m2 : module EV) : nat → m1.(m_state) -> list (event EV) -> Prop :=
 | Wp_step' σi1 κs n:
@@ -425,9 +559,6 @@ Proof.
     eexists. by apply: has_trace_trans.
   - move => ??? /Hinvsafe ? σs ?. exists σs. naive_solver.
 Qed.
-
-Definition has_no_behavior {EV} (m : module EV) (σ : m.(m_state)) :=
-  ∀ σ' κs, has_trace m σ κs σ' → κs = [].
 
 Lemma inv_implies_refines' {EV} (m1 m2 : module EV) (inv : m1.(m_state) → m2.(m_state) → Prop):
   inv m1.(m_initial) m2.(m_initial) →
